TestVectorsAwsCryptographicMaterialProviders/runtimes/net/Generated/KeyVectors/KeyDescription.cs
@@ -9,7 +9,9 @@ using System;
  private AWS.Cryptography.MaterialProvidersTestVectorKeys.KmsMrkAwareDiscovery _kmsMrkDiscovery ;
  private AWS.Cryptography.MaterialProvidersTestVectorKeys.RawRSA _rSA ;
  private AWS.Cryptography.MaterialProvidersTestVectorKeys.RawAES _aES ;
- private AWS.Cryptography.MaterialProvidersTestVectorKeys.InvalidKeyring _invalid ;
+ private AWS.Cryptography.MaterialProvidersTestVectorKeys.StaticKeyring _static ;
+ private AWS.Cryptography.MaterialProvidersTestVectorKeys.KmsRsaKeyring _kmsRsa ;
+ private AWS.Cryptography.MaterialProvidersTestVectorKeys.HierarchyKeyring _hierarchy ;
  public AWS.Cryptography.MaterialProvidersTestVectorKeys.KMSInfo Kms {
  get { return this._kms; }
  set { this._kms = value; }
@@ -45,12 +47,26 @@ using System;
  public bool IsSetAES () {
  return this._aES != null;
 }
- public AWS.Cryptography.MaterialProvidersTestVectorKeys.InvalidKeyring Invalid {
- get { return this._invalid; }
- set { this._invalid = value; }
+ public AWS.Cryptography.MaterialProvidersTestVectorKeys.StaticKeyring Static {
+ get { return this._static; }
+ set { this._static = value; }
 }
- public bool IsSetInvalid () {
- return this._invalid != null;
+ public bool IsSetStatic () {
+ return this._static != null;
+}
+ public AWS.Cryptography.MaterialProvidersTestVectorKeys.KmsRsaKeyring KmsRsa {
+ get { return this._kmsRsa; }
+ set { this._kmsRsa = value; }
+}
+ public bool IsSetKmsRsa () {
+ return this._kmsRsa != null;
+}
+ public AWS.Cryptography.MaterialProvidersTestVectorKeys.HierarchyKeyring Hierarchy {
+ get { return this._hierarchy; }
+ set { this._hierarchy = value; }
+}
+ public bool IsSetHierarchy () {
+ return this._hierarchy != null;
 }
  public void Validate() {
  var numberOfPropertiesSet = Convert.ToUInt16(IsSetKms()) +
@@ -58,7 +74,9 @@ using System;
  Convert.ToUInt16(IsSetKmsMrkDiscovery()) +
  Convert.ToUInt16(IsSetRSA()) +
  Convert.ToUInt16(IsSetAES()) +
- Convert.ToUInt16(IsSetInvalid()) ;
+ Convert.ToUInt16(IsSetStatic()) +
+ Convert.ToUInt16(IsSetKmsRsa()) +
+ Convert.ToUInt16(IsSetHierarchy()) ;
  if (numberOfPropertiesSet == 0) throw new System.ArgumentException("No union value set");
 
  if (numberOfPropertiesSet > 1) throw new System.ArgumentException("Multiple union values set");
