TestVectorsAwsCryptographicMaterialProviders/dafny/KeyVectors/src/KeyDescription.dfy
@@ -21,64 +21,64 @@ module {:options "-functionSyntax:4"} KeyDescription {
     var typ :- GetString(typString, obj);
 
     :- Need(KeyDescriptionString?(typ), "Unsupported KeyDescription type:" + typ);
+    var key :- GetString("key", obj);
+
     match typ
+    case "static-material" =>
+      Success(Static(StaticKeyring( keyId := key )))
+    case "aws-kms" =>
+      Success(Kms(KMSInfo( keyId := key )))
+    case "aws-kms-mrk-aware" =>
+      Success(KmsMrk(KmsMrkAware( keyId := key )))
     case "aws-kms-mrk-aware-discovery" =>
-      var defaultMrkRegion :- GetString("default-mrk-region", obj);
-      var awsKmsDiscoveryFilter :- ToDiscoveryFilter(obj);
+      var defaultMrkRegion :- GetString("partition", obj);
+      var filter := GetObject("aws-kms-discovery-filter", obj);
+      var awsKmsDiscoveryFilter := ToDiscoveryFilter(obj);
       Success(KmsMrkDiscovery(KmsMrkAwareDiscovery(
                                 keyId := "aws-kms-mrk-aware-discovery",
                                 defaultMrkRegion := defaultMrkRegion,
                                 awsKmsDiscoveryFilter := awsKmsDiscoveryFilter
                               )))
-    case _ =>
-      var key :- GetString("key", obj);
-      match typ
-      case "static-material" =>
-        Success(Static(StaticKeyring( keyId := key )))
-      case "aws-kms" =>
-        Success(Kms(KMSInfo( keyId := key )))
-      case "aws-kms-mrk-aware" =>
-        Success(KmsMrk(KmsMrkAware( keyId := key )))
-      case "raw" =>
-        var algorithm :- GetString("encryption-algorithm", obj);
-        var providerId :- GetString("provider-id", obj);
-        :- Need(RawAlgorithmString?(algorithm), "Unsupported algorithm:" + algorithm);
-        match algorithm
-        case "aes" =>
-          Success(AES(RawAES( keyId := key, providerId := providerId )))
-        case "rsa" =>
-          var paddingAlgorithm :- GetString("padding-algorithm", obj);
-          var paddingHash :- GetString("padding-hash", obj);
-          :- Need(PaddingAlgorithmString?(paddingAlgorithm), "Unsupported paddingAlgorithm:" + paddingAlgorithm);
-          :- Need(PaddingHashString?(paddingHash), "Unsupported paddingHash:" + paddingHash);
+    case "aws-kms-rsa" =>
+      Success(KmsRsa(KmsRsaKeyring( keyId := key )))
+    case "aws-kms-hierarchy" =>
+      Success(Hierarchy(HierarchyKeyring( keyId := key )))
+    case "raw" =>
+      var algorithm :- GetString("encryption-algorithm", obj);
+      var providerId :- GetString("provider-id", obj);
+      :- Need(RawAlgorithmString?(algorithm), "Unsupported algorithm:" + algorithm);
+      match algorithm
+      case "aes" =>
+        Success(AES(RawAES( keyId := key, providerId := providerId )))
+      case "rsa" =>
+        var paddingAlgorithm :- GetString("padding-algorithm", obj);
+        var paddingHash :- GetString("padding-hash", obj);
+        :- Need(PaddingAlgorithmString?(paddingAlgorithm), "Unsupported paddingAlgorithm:" + paddingAlgorithm);
+        :- Need(PaddingHashString?(paddingHash), "Unsupported paddingHash:" + paddingHash);
 
-          match paddingAlgorithm
-          case "pkcs1" =>
-            :- Need(paddingHash == "sha1", "Unsupported padding with pkcs1:" + paddingHash);
-            Success(RSA(RawRSA( keyId := key, providerId := providerId, padding := AwsCryptographyMaterialProvidersTypes.PKCS1 )))
-          case "oaep-mgf1" => match paddingHash
-            case "sha1" => Success(RSA(RawRSA( keyId := key, providerId := providerId, padding := AwsCryptographyMaterialProvidersTypes.OAEP_SHA1_MGF1 )))
-            case "sha256" => Success(RSA(RawRSA( keyId := key, providerId := providerId, padding := AwsCryptographyMaterialProvidersTypes.OAEP_SHA256_MGF1 )))
-            case "sha384" => Success(RSA(RawRSA( keyId := key, providerId := providerId, padding := AwsCryptographyMaterialProvidersTypes.OAEP_SHA384_MGF1 )))
-            case "sha512" => Success(RSA(RawRSA( keyId := key, providerId := providerId, padding := AwsCryptographyMaterialProvidersTypes.OAEP_SHA512_MGF1 )))
+        match paddingAlgorithm
+        case "pkcs1" =>
+          :- Need(paddingHash == "sha1", "Unsupported padding with pkcs1:" + paddingHash);
+          Success(RSA(RawRSA( keyId := key, providerId := providerId, padding := AwsCryptographyMaterialProvidersTypes.PKCS1 )))
+        case "oaep-mgf1" => match paddingHash
+          case "sha1" => Success(RSA(RawRSA( keyId := key, providerId := providerId, padding := AwsCryptographyMaterialProvidersTypes.OAEP_SHA1_MGF1 )))
+          case "sha256" => Success(RSA(RawRSA( keyId := key, providerId := providerId, padding := AwsCryptographyMaterialProvidersTypes.OAEP_SHA256_MGF1 )))
+          case "sha384" => Success(RSA(RawRSA( keyId := key, providerId := providerId, padding := AwsCryptographyMaterialProvidersTypes.OAEP_SHA384_MGF1 )))
+          case "sha512" => Success(RSA(RawRSA( keyId := key, providerId := providerId, padding := AwsCryptographyMaterialProvidersTypes.OAEP_SHA512_MGF1 )))
   }
 
   function ToDiscoveryFilter(obj: seq<(string, JSON)>)
-    : Result<Option<AwsCryptographyMaterialProvidersTypes.DiscoveryFilter>, string>
+    : Option<AwsCryptographyMaterialProvidersTypes.DiscoveryFilter>
   {
-    var filter := GetObject("aws-kms-discovery-filter", obj).ToOption();
-    if filter.Some? then
-      var partition :- GetString("partition", filter.value);
-      var accountIds :- GetArrayString("account-ids", filter.value);
-      Success(Some(AwsCryptographyMaterialProvidersTypes.DiscoveryFilter(
-                     partition := partition,
-                     accountIds := accountIds
-                   )))
-    else
-      Success(None)
+    var filter :- GetObject("aws-kms-discovery-filter", obj).ToOption();
+    var partition :- GetString("partition", filter).ToOption();
+    var accountIds :- GetArrayString("account-ids", filter).ToOption();
+    Some(AwsCryptographyMaterialProvidersTypes.DiscoveryFilter(
+           partition := partition,
+           accountIds := accountIds
+         ))
   }
 
-  type KeyDescriptionString = s: string | KeyDescriptionString?(s) witness *
   predicate KeyDescriptionString?(s: string)
   {
     || s == "static-material"
@@ -86,23 +86,22 @@ module {:options "-functionSyntax:4"} KeyDescription {
     || s == "aws-kms-mrk-aware"
     || s == "aws-kms-mrk-aware-discovery"
     || s == "raw"
+    || s == "aws-kms-hierarchy"
+    || s == "aws-kms-rsa"
   }
 
-  type RawAlgorithmString = s: string | RawAlgorithmString?(s) witness *
   predicate RawAlgorithmString?(s: string)
   {
     || s == "aes"
     || s == "rsa"
   }
 
-  type PaddingAlgorithmString = s: string | PaddingAlgorithmString?(s) witness *
   predicate PaddingAlgorithmString?(s: string)
   {
     || s == "pkcs1"
     || s == "oaep-mgf1"
   }
 
-  type PaddingHashString = s: string | PaddingHashString?(s) witness *
   predicate PaddingHashString?(s: string)
   {
     || s == "sha1"
